testing fshift_div in vcfloat.v

leapfrog_project/vcfloat.v
@@ -121,7 +121,9 @@ Ltac vcfloat_simplifications :=
   repeat change (cast_lub_l Tsingle Tsingle ?A) with A; 
   repeat change (cast_lub_l Tdouble Tdouble ?A) with A; 
   repeat change (cast_lub_r Tsingle Tsingle ?A) with A; 
-  repeat change (cast_lub_r Tdouble Tdouble ?A) with A.
+  repeat change (cast_lub_r Tdouble Tdouble ?A) with A;
+  repeat change (cast Tdouble Tdouble ?A) with A;
+  repeat change (cast Tsingle Tsingle ?A) with A.
 
 Ltac focus f :=
  match goal with |- context [f ?a] =>
@@ -210,6 +212,9 @@ Ltac simplify_fshift :=
 Definition optimize {V: Type} {NANS: Nans} (e: expr) : expr :=
   @fshift V NANS (@fcval V NANS e).
 
+Definition optimize_div {V: Type} {NANS: Nans} (e: expr) : expr :=
+  @fshift_div V NANS (@fshift V NANS (@fcval V NANS e)).
+
 Ltac simplify_opt e1 :=
   match e1 with (optimize ?e) =>   
   unfold optimize;
@@ -252,6 +257,73 @@ Definition _v : AST.ident := 7%positive.
 Definition e1 := ltac:(let e' := HO_reify_float_expr constr:([_x; _v]) leapfrog_stepx in exact e').
 Definition e :=  ltac:(let e' := reify_float_expr constr:( (float32_of_Z (-1))%F32 ) in exact e').
 Definition e2 := ltac:(let e' := HO_reify_float_expr constr:([_x]) F in exact e').
+
+Goal optimize_div e1 = Var Tsingle _x.
+  unfold optimize_div. 
+  let e' := eval hnf in e1 in change e1 with e'.
+       cbv beta fix iota zeta delta [FPLangOpt.fcval FPLangOpt.fcval_nonrec 
+                    FPLangOpt.option_pair_of_options];
+     vcfloat_compute.
+     cbv beta fix iota delta [FPLangOpt.fshift FPLangOpt.fcval_nonrec ].
+     vcfloat_simplifications.
+repeat match goal with
+| |- context [binop_eqb ?a  ?b] =>
+      simplify_float_ops (binop_eqb a b)
+end.      
+ cbv beta iota zeta.
+repeat match goal with
+| |- context [to_power_2 ?a] =>
+      simplify_float_ops (to_power_2 a) 
+| |- context [to_power_2_pos ?a] =>
+      simplify_float_ops (to_power_2_pos a) 
+| |- context [binary_float_eqb ?a  ?b] =>
+      simplify_float_ops (binary_float_eqb a b)
+| |- context [to_inv_power_2 ?a] =>
+      simplify_float_ops (to_inv_power_2 a) 
+end. 
+
+cbv beta iota zeta.
+
+cbv beta fix iota delta [FPLangOpt.fshift_div FPLangOpt.fcval_nonrec].
+vcfloat_simplifications.
+repeat match goal with
+| |- context [binop_eqb ?a  ?b] =>
+      simplify_float_ops (binop_eqb a b)
+end.
+cbv beta iota zeta.
+repeat match goal with
+| |- context [to_power_2 ?a] =>
+      simplify_float_ops (to_power_2 a) 
+| |- context [to_power_2_pos ?a] =>
+      simplify_float_ops (to_power_2_pos a) 
+| |- context [binary_float_eqb ?a  ?b] =>
+      simplify_float_ops (binary_float_eqb a b)
+| |- context [to_inv_power_2 ?a] =>
+      simplify_float_ops (to_inv_power_2 a) 
+end. 
+vcfloat_simplifications.
+
+match goal with
+|- context [Bexact_inverse] =>
+cbv [Bexact_inverse ];
+match goal with
+|- context [Pos.eq_dec ?a ?b] =>
+      simplify_float_ops (Pos.eq_dec a b); cbv beta iota zeta
+end
+end. 
+
+repeat match goal with
+|- context [Z_le_dec ?a ?b] =>
+      simplify_float_ops (Z_le_dec a b); cbv beta iota zeta
+end.
+
+repeat match goal with
+|- context [binary_float_eqb ?a  ?b] =>
+      simplify_float_ops (binary_float_eqb a b)
+end.
+
+cbv beta iota zeta.  
+
 
 Goal optimize e1 = Var Tsingle _x.
 simplify_opt (optimize e1).
